

GRAMMARS

1. Given the grammar $G = (N, \Sigma, P, S)$

$$N = \{S, C\}$$

$$\Sigma = \{a, b\}$$

$$P : S \rightarrow ab \mid aCSb$$

$$C \rightarrow S \mid bSb$$

$$CS \rightarrow b,$$

prove that $w = ab(ab^2)^2 \in L(G)$.

$$Obs. : (ab)^2 = abab \neq a^2b^2 = aabb$$

Sol.

$$\begin{array}{ccccccc} & & & & 2 & & \\ S & \Rightarrow & aCSb & \Rightarrow & abSbSb & \Rightarrow & ababbabb \\ (2) & & (4) & & (1) & & \end{array}$$

$$\begin{array}{c} 4 \\ \Rightarrow S \Rightarrow ababbabb = w \Rightarrow w \in L(G) \end{array}$$

2. Given the grammar $G = (N, \Sigma, P, S)$

$$N = \{S\}$$

$$\Sigma = \{a, b, c\}$$

$$P : S \rightarrow a^2S \mid bc,$$

find $L(G)$.

Sol.

$$\text{Let } L = \{a^{2n}bc \mid n \in \mathbb{N}\}$$

$$? L = L(G)$$

(1) ? $L \subseteq L(G)$ (all sequences of that shape are generated by G)

$$? \forall n \in \mathbb{N}, a^{2n}bc \in L(G)$$

Take $P(n): a^{2n}bc \in L(G)$ and prove $P(n)$ true, $\forall n \in \mathbb{N}$

We'll prove by mathematical induction

(a) Verification step: $? P(0): a^0bc \in L(G)$ is true

$$S \Rightarrow bc = a^0bc \Rightarrow P(0) \text{ true}$$

(2)

(b) Proof step: We suppose $P(k)$ is true and then prove that $P(k+1)$ is also true, where $k \in \mathbb{N}$

$$\begin{array}{c} * \\ P(k) \text{ true} \Rightarrow a^{2k}bc \in L(G) \Rightarrow S \Rightarrow a^{2k}bc \text{ (induction hypothesis)} \end{array}$$

$$\begin{array}{c} * \\ S \Rightarrow a^2S \Rightarrow a^2a^{2k}bc = a^{2(k+1)}bc \\ (1) \quad (\text{ind. hypo.}) \end{array}$$

$$\begin{array}{c} * \\ \Rightarrow S \Rightarrow a^{2(k+1)}bc \Rightarrow P(k+1) \text{ is true} \end{array}$$

(a) + (b) \Rightarrow (1)

(2) $? L \supseteq L(G)$ (G generates **only** sequences of that shape)

$$\begin{array}{l} S \Rightarrow bc = a^0bc \\ \Rightarrow a^2S \Rightarrow a^2bc \\ \Rightarrow a^4S \Rightarrow a^4bc \\ \Rightarrow a^6S \Rightarrow \dots \end{array}$$

We notice that starting from S and using **all** grammar productions in **all** possible combinations, we only get, as sequences of terminals,

sequences of the shape $a^{2^n}bc$ where $n \in \mathbb{N}$. It follows that the grammar doesn't generate anything else.

Obs.: This inclusion may also be discharged by induction.

3. Find a grammar that generates $L = \{0^n 1^n 2^m \mid n, m \in \mathbb{N}^*\}$

Sol.

$$G = (N, \Sigma, P, S)$$

$$N = \{S, V, C\}$$

$$\Sigma = \{0, 1, 2\}$$

$$P : S \rightarrow VC$$

$$V \rightarrow 0V1 \mid 01$$

$$C \rightarrow 2 \mid 2C$$

$$(1) ? L \subseteq L(G)$$

$$? \forall n, m \in \mathbb{N}^*, 0^n 1^n 2^m \in L(G)$$

$$\text{Let } n, m \in \mathbb{N}^*$$

$$\begin{array}{ccccccc} & n & & m & & * & \\ S & \Rightarrow & VC & \Rightarrow & 0^n 1^n C & \Rightarrow & 0^n 1^n 2^m \Rightarrow S \Rightarrow 0^n 1^n 2^m \Rightarrow 0^n 1^n 2^m \in L(G) \\ (1) & (a) & & (b) & & & \end{array}$$

$$(a) V \Rightarrow 0^n 1^n, \forall n \in \mathbb{N}^*$$

$$(b) C \Rightarrow 2^m, \forall m \in \mathbb{N}^*$$

HW: Prove (a) and (b) above by induction

Justify the reverse inclusion